Minor changes

ref_impl/src/verifier/expression_expr.ts
@@ -7,51 +7,53 @@ import { VarTerm, TermExpr } from "./term_expr";
 
 abstract class ExprExpr {
     readonly tabSymbol = "    ";
-    abstract toML(indentatioLevel : number): string;
+    abstract toML(indentatioLevel: number): string;
 }
 
 class ReturnExpr extends ExprExpr {
-    readonly returnExpr : TermExpr;
-    constructor(returnExpr : TermExpr){
+    readonly returnExpr: TermExpr;
+    constructor(returnExpr: TermExpr) {
         super();
         this.returnExpr = returnExpr;
     }
-    toML(indentatioLevel : number){
+    toML(indentatioLevel: number) {
         return this.tabSymbol.repeat(indentatioLevel) + this.returnExpr.toML();
     }
 }
 
 class AssignmentExpr extends ExprExpr {
-    readonly lhs : VarTerm;
-    readonly rhs : TermExpr;
-    readonly continuation : ExprExpr;
-    constructor(lhs : VarTerm, rhs : TermExpr, continuation : ExprExpr){
+    readonly lhs: VarTerm;
+    readonly rhs: TermExpr;
+    readonly continuation: ExprExpr;
+    constructor(lhs: VarTerm, rhs: TermExpr, continuation: ExprExpr) {
         super();
         this.lhs = lhs;
         this.rhs = rhs;
         this.continuation = continuation;
     }
-    toML(indentatioLevel : number){
-        return this.tabSymbol.repeat(indentatioLevel) + "let " + this.lhs.toML() + " = " + this.rhs.toML() + " in \n" 
-        + this.continuation.toML(indentatioLevel + 1);
+    toML(indentatioLevel: number) {
+        return this.tabSymbol.repeat(indentatioLevel)
+            + "let " + this.lhs.toML() + " = " + this.rhs.toML() + " in \n"
+            + this.continuation.toML(indentatioLevel + 1);
     }
 }
 
 class ConditionalExpr extends ExprExpr {
-    readonly condition : TermExpr;
-    readonly ifBranch : ExprExpr;
-    readonly elseBranch : ExprExpr;
-    constructor(condition : TermExpr, ifBranch : ExprExpr, elseBranch : ExprExpr){
+    readonly condition: TermExpr;
+    readonly ifBranch: ExprExpr;
+    readonly elseBranch: ExprExpr;
+    constructor(condition: TermExpr, ifBranch: ExprExpr, elseBranch: ExprExpr) {
         super();
         this.condition = condition;
         this.ifBranch = ifBranch;
         this.elseBranch = elseBranch;
     }
-    toML(indentatioLevel : number){
-        return this.tabSymbol.repeat(indentatioLevel) + "if " + this.condition.toML() + " then \n" 
-        + this.ifBranch.toML(indentatioLevel + 1) + "\n" 
-        + this.tabSymbol.repeat(indentatioLevel) + "else \n" 
-        + this.elseBranch.toML(indentatioLevel + 1);
+    toML(indentatioLevel: number) {
+        return this.tabSymbol.repeat(indentatioLevel)
+            + "if " + this.condition.toML() + " then \n"
+            + this.ifBranch.toML(indentatioLevel + 1) + "\n"
+            + this.tabSymbol.repeat(indentatioLevel) + "else \n"
+            + this.elseBranch.toML(indentatioLevel + 1);
     }
 }
 
