ref_impl/NSMain__main_main.fst
@@ -1,23 +1,24 @@
 module NSMain__main_main
 
-val nSMain__max0 : bool -> bool -> Tot bool
+val nSMain__max0 : int -> int -> Tot int
 let nSMain__max0 x y = 
-    if (op_Equality x true) then 
-        let _ir_ret__1 = y in 
-            let _ir_ret__2 = _ir_ret__1 in 
-                let _return_ = _ir_ret__2 in 
-                    _return_
-    else 
-        let _ir_ret_ = x in 
-            let _ir_ret__2 = _ir_ret_ in 
-                let _return_ = _ir_ret__2 in 
-                    _return_
+    let __tmp_0 = (op_GreaterThanOrEqual x y) in 
+        if (op_Equality __tmp_0 true) then 
+            let _ir_ret__1 = x in 
+                let _ir_ret__2 = _ir_ret__1 in 
+                    let _return_ = _ir_ret__2 in 
+                        _return_
+        else 
+            let _ir_ret_ = y in 
+                let _ir_ret__2 = _ir_ret_ in 
+                    let _return_ = _ir_ret__2 in 
+                        _return_
 
-val nSMain__main : bool
+val nSMain__main : int
 let nSMain__main  = 
     let x = 10 in 
         let y = 20 in 
-            let __tmp_2 = (nSMain__max0 true false) in 
+            let __tmp_2 = (nSMain__max0 x y) in 
                 let z = __tmp_2 in 
                     let _ir_ret_ = z in 
                         let _return_ = _ir_ret_ in 
